proof/RUSC.v
@@ -2,14 +2,8 @@
 Require Import String.
 Require Import CoqlibC Errors ErrorsC.
 Require Import AST Linking Smallstep.
-(** Command-line flags. *)
-Require Import Compopts.
 (** newly added **)
-Require Import BehaviorsC.
-Require Export Compiler.
-Require Import Simulation.
-Require Import Sem SimProg Skeleton Mod ModSem SimMod SimModSem SimSymb SimMem Sound SimSymb.
-Require Import SemProps AdequacyLocal.
+Require Import BehaviorsC Sem.
 
 
 Module program_relation.
@@ -141,83 +135,3 @@ Proof.
   eapply RU; eauto; eapply self_related_mon; eauto.
 Qed.
 Hint Resolve rusc_mon.
-
-Program Definition mkPR (MR: SimMem.class) (SR: SimSymb.class MR) (MP: Sound.class)
-  : program_relation.t := program_relation.mk
-                            (fun (p_src p_tgt: program) =>
-                               forall (WF: forall x (IN: In x p_src), Sk.wf x),
-                               exists pp,
-                                 (<<SIMS: @ProgPair.sim MR SR MP pp>>)
-                                 /\ (<<SRCS: pp.(ProgPair.src) = p_src>>)
-                                 /\ (<<TGTS: pp.(ProgPair.tgt) = p_tgt>>)) _ _ _.
-Next Obligation.
-  exploit REL0; eauto. { i. eapply WF. rewrite in_app_iff. eauto. } intro T0; des.
-  exploit REL1; eauto. { i. eapply WF. rewrite in_app_iff. eauto. } intro T1; des.
-  clarify. unfold ProgPair.sim in *. rewrite Forall_forall in *. eexists (_ ++ _). esplits; eauto.
-  - rewrite Forall_forall in *. i. rewrite in_app_iff in *. des; [apply SIMS|apply SIMS0]; eauto.
-  - unfold ProgPair.src. rewrite map_app. ss.
-  - unfold ProgPair.tgt. rewrite map_app. ss.
-Qed.
-Next Obligation.
-  destruct (classic (forall x (IN: In x p_src), Sk.wf x)) as [WF|NWF]; cycle 1.
-  { eapply sk_nwf_improves; auto. }
-  eapply bsim_improves.
-  eapply mixed_to_backward_simulation.
-  specialize (REL WF). des. clarify.
-  eapply (@adequacy_local MR SR MP). auto.
-Qed.
-Next Obligation. exists []. splits; ss. Qed.
-
-
-Definition relate_single (MR: SimMem.class) (SR: SimSymb.class MR) (MP: Sound.class)
-           (p_src p_tgt: Mod.t) : Prop :=
-  forall (WF: Sk.wf p_src),
-  exists mp,
-    (<<SIM: @ModPair.sim MR SR MP mp>>)
-    /\ (<<SRC: mp.(ModPair.src) = p_src>>)
-    /\ (<<TGT: mp.(ModPair.tgt) = p_tgt>>).
-Arguments relate_single : clear implicits.
-
-Lemma relate_single_program MR SR MP p_src p_tgt
-      (REL: relate_single MR SR MP p_src p_tgt):
-    (mkPR MR SR MP) [p_src] [p_tgt].
-Proof.
-  unfold relate_single. ss. i.
-  exploit REL; [ss; eauto|]. i. des. clarify.
-  exists [mp]. esplits; ss; eauto.
-Qed.
-Arguments relate_single_program : clear implicits.
-
-Lemma relate_each_program MR SR MP
-      (p_src p_tgt: program)
-      (REL: Forall2 (relate_single MR SR MP) p_src p_tgt):
-    (mkPR MR SR MP) p_src p_tgt.
-Proof.
-  revert p_tgt REL. induction p_src; ss; i.
-  - inv REL. exists []; splits; ss.
-  - inv REL. exploit IHp_src; eauto. i. des.
-    exploit H1; eauto. i. des. clarify.
-    exists (mp :: pp); splits; ss. econs; eauto.
-Qed.
-Arguments relate_each_program : clear implicits.
-
-Lemma relate_single_rtc_rusc (R: program_relation.t -> Prop) MR SR MP
-      (p_src p_tgt: Mod.t)
-      (REL: rtc (relate_single MR SR MP) p_src p_tgt)
-      (RELIN: R (mkPR MR SR MP)):
-    rusc R [p_src] [p_tgt].
-Proof.
-  induction REL; try refl.
-  - etrans; eauto. eapply rusc_incl; eauto. eapply relate_single_program; eauto.
-Qed.
-Arguments relate_single_program : clear implicits.
-
-Lemma relate_single_rusc (R: program_relation.t -> Prop) MR SR MP
-      (p_src p_tgt: Mod.t)
-      (REL: (relate_single MR SR MP) p_src p_tgt)
-      (RELIN: R (mkPR MR SR MP)):
-    rusc R [p_src] [p_tgt].
-Proof.
-  eapply relate_single_rtc_rusc; eauto. eapply rtc_once. eauto.
-Qed.
-Arguments relate_single_program : clear implicits.
